Linglib.lean
@@ -2993,3 +2993,4 @@ import Linglib.Data.Examples.Ariel2001
 import Linglib.Data.Examples.AsherLascarides2003
 import Linglib.Data.Examples.AssmannEtAl2023
 import Linglib.Data.Examples.Asudeh2022
+import Linglib.Data.Examples.AugurzkyEtAl2023
